----
$$
\frac{1}{4\pi\epsilon_{0}}\cdot \frac{e^{2}}{r^{2}} = \frac{m_{e}v^{2}}{r}
$$
$$
m_{e}vr = n\hbar
$$
$$
v = \frac{n\hbar}{m_{e}r}
$$
$$
\frac{1}{4\pi\epsilon_{0}}\cdot \frac{e^{2}}{r^{2}} = \frac{m_{e}(\frac{n\hbar}{m_{e}r})^{2}}{r}
$$
$$
\frac{1}{4\pi\epsilon_{0}}\cdot e^{2} = \frac{n^{2}\hbar^{2}}{m_{e}r} 
$$
$$
r_{n} = \frac{4\pi\epsilon_{0}n^{2}\hbar^{2}}{m_{e}e^{2}}
$$
$$
r_{1} = a_{0} = 0.529 \dot{A} (10^{-10}m)
$$
$$
K = \frac{1}{2}m_{e}v^{2}
$$
$$
K = \frac{1}{2} \cdot \frac{1}{4\pi\epsilon_{0}}\cdot \frac{e^{2}}{r}
$$
$$
U = - \frac{1}{4\pi\epsilon_{0}}\cdot \frac{e^{2}}{r}
$$
$$
E = K + U = -\frac{1}{2}\cdot \frac{1}{4\pi\epsilon_{0}}\cdot \frac{e^{2}}{r}
$$
$$
r_{n} = \frac{4\pi\epsilon_{0}n^{2}\hbar^{2}}{m_{e}e^{2}}
$$
$$
E_{n} = -\frac{1}{2}\cdot \frac{1}{4\pi\epsilon_{0}}\cdot \frac{e^{2}}{ \frac{4\pi\epsilon_{0}n^{2}\hbar^{2}}{m_{e}e^{2}}}
$$
$$
E_{n} = -\frac{m_{e}e^{4}}{8\epsilon^{2}_{0}h^{2}}\cdot \frac{1}{n^{2}} \simeq -\frac{13.6}{n^{2}} eV
$$
$$
R_{\infty} = \frac{m_{e}e^{4}}{8\epsilon^{2}_{0}h^{3}c}
$$
$$
R_{H} = R_{\infty} \frac{\mu}{m_{e}}
$$
$$
\mu = \frac{m_{e}m_{p}}{m_{e} + m_{p}}
$$
$$
E_{n} = -hcR_{\infty} \frac{1}{n^{2}}
$$
$$
\Delta E = E_{n+1} - E_{n} = h\nu = \frac{hc}{\lambda} = hcR_{\infty}\left[ \frac{1}{n^{2}} - \frac{1}{(n+1)^2} \right] 
$$
$$
\frac{1}{\lambda} = R_{\infty}\left[ \frac{1}{n^{2}} - \frac{1}{(n+1)^{2}} \right]
$$
$$
\frac{1}{\lambda} = R_{\infty}\left[ \frac{1}{2^{2}} - \frac{1}{(n)^{2}} \right]; n\geq 3
$$